wip

fixedpoints.thy
@@ -134,7 +134,76 @@ proof -
 
 
     oops
+(*
+definition lfp2 :: "(('a \<Rightarrow> bool) \<Rightarrow> ('a \<Rightarrow> bool)) \<Rightarrow> ('a \<Rightarrow> bool)" where
+"lfp2 f \<equiv> SUP i. (f ^^ i) bot"
 
+
+lemma lfp2_fixpoint:
+  assumes mono: "mono f"
+  shows "f (lfp2 f) = lfp2 f"
+  apply (auto simp add: lfp2_def)
+proof (rule antisym)
+  show "(SUP i. (f ^^ i) bot) \<le> f (SUP i. (f ^^ i) bot)"
+    using [[smt_solver=cvc4]]
+    by (smt SUP_least Sup_le_iff assms bot_least funpow_swap1 monoD mono_def mono_pow order_refl order_trans range_eqI)
+
+  show "f (SUP i. (f ^^ i) bot) \<le> (SUP i. (f ^^ i) bot)"
+
+
+
+lemma lfp2_to_iterate:
+  fixes f :: "('a \<Rightarrow> bool) \<Rightarrow> 'a \<Rightarrow> bool"
+  assumes lfp_x: "lfp2 f x"
+    and mono: "mono f"
+  shows "\<exists>i. (f ^^ i) bot x"
+  oops
+*)
+
+(*
+definition lfp2 :: "(('a \<Rightarrow> bool) \<Rightarrow> ('a \<Rightarrow> bool)) \<Rightarrow> ('a \<Rightarrow> bool)" where
+"lfp2 f \<equiv> \<lambda>x. \<exists>i. (f ^^ i) bot x"
+
+lemma lfp2_to_iterate:
+  fixes f :: "('a \<Rightarrow> bool) \<Rightarrow> 'a \<Rightarrow> bool"
+  assumes lfp_x: "lfp2 f x"
+  shows "\<exists>i. (f ^^ i) bot x"
+  by (meson lfp2_def lfp_x)
+
+
+
+
+thm lfp_fixpoint
+
+lemma lfp2_fixpoint:
+  assumes "mono f"
+  shows "f (lfp2 f) = lfp2 f"
+  unfolding lfp2_def
+proof (auto intro!: ext)
+
+
+  show "\<exists>i. (f ^^ i) bot x"
+    if c0: "f (\<lambda>x. \<exists>i. (f ^^ i) bot x) x"
+    for  x
+
+    sorry
+
+  show "f (\<lambda>x. \<exists>i. (f ^^ i) bot x) x"
+    if c0: "(f ^^ i) bot x"
+    for  x i
+    sorry
+qed
+
+
+
+
+
+lemma lfp2_unfold:
+  assumes "mono f"
+  shows "lfp2 f = f (lfp2 f)"
+  by (simp add: assms lfp2_fixpoint)
+
+*)
 
 
 end
