invariant_simps.thy
@@ -25,11 +25,11 @@ definition
 
 lemma i_invocationOp_simps:
   "(i_invocationOp (invContextH state_callOrigin state_transactionOrigin state_transactionStatus state_happensBefore 
-   state_calls state_knownIds state_invocationOp state_invocationRes vis) r \<triangleq> Op) \<longleftrightarrow> (state_invocationOp r \<triangleq> Op)"
+   state_calls state_knownIds state_invocationOp state_invocationRes ) r \<triangleq> Op) \<longleftrightarrow> (state_invocationOp r \<triangleq> Op)"
   by (auto simp add: invContextH_def)
 
 lemma invocation_happensBefore_simps:
-  "((x,y) \<in> invocation_happensBefore (invContextH state_callOrigin state_transactionOrigin ts state_happensBefore cs ki io ir vis)) 
+  "((x,y) \<in> invocation_happensBefore (invContextH state_callOrigin state_transactionOrigin ts state_happensBefore cs ki io ir )) 
 \<longleftrightarrow> ((\<exists>c t. state_callOrigin c \<triangleq> t \<and> state_transactionOrigin t \<triangleq> x) 
         \<and> (\<exists>c t.  state_callOrigin c \<triangleq> t \<and> state_transactionOrigin t \<triangleq> y) 
         \<and> (\<forall>cx tx cy ty. state_callOrigin cx \<triangleq> tx \<and> state_transactionOrigin tx \<triangleq> x
